meta-theory/pure_obs_sem_equalScript.sml
@@ -1,0 +1,119 @@
+(*
+   This file proves that bisimilar (≃) expressions lead to equal (=)
+   observational semantics:
+
+       ∀x y. x ≃ y ⇒ semantics x [] = semantics y []
+
+*)
+open HolKernel Parse boolLib bossLib term_tactic;
+open fixedPointTheory arithmeticTheory listTheory stringTheory alistTheory
+     optionTheory pairTheory ltreeTheory llistTheory bagTheory
+     BasicProvers pred_setTheory relationTheory rich_listTheory finite_mapTheory
+     dep_rewrite io_treeTheory;
+open pure_expTheory pure_valueTheory pure_evalTheory pure_eval_lemmasTheory
+     pure_exp_lemmasTheory pure_exp_relTheory pure_semanticsTheory;
+
+val _ = new_theory "pure_obs_sem_equal";
+
+Triviality eval_wh_Cons:
+  wh_Constructor n es = eval_wh x ∧ x ≃ y ⇒
+  ∃es1. eval_wh y = wh_Constructor n es1 ∧ LIST_REL (≃) es es1
+Proof
+  fs [Once app_bisimilarity_iff]
+  \\ Cases_on ‘eval_wh x’ \\ fs []
+  \\ rw [] \\ gvs []
+  \\ cheat
+QED
+
+Theorem next_lemma[local]:
+  ∀a res1.
+    next a res1 ⇒
+    ∀x xs y ys.
+      a = (eval_wh x,xs) ∧ x ≃ y ∧ LIST_REL (≃) xs ys ⇒
+      ∃res2. next (eval_wh y,ys) res2 ∧
+             (res1 ≠ res2 ⇒
+                ∃a new1 new2. res1 = Act a new1 ∧
+                              res2 = Act a new2 ∧
+                              LIST_REL (≃) new1 new2)
+Proof
+  ho_match_mp_tac next_ind \\ rw [] \\ fs [PULL_EXISTS]
+  THEN1
+   (qsuff_tac ‘∃e1. eval_wh y = wh_Constructor "Act" [e1] ∧ eval_wh e1 = wh_Atom a’
+    THEN1 (rw [] \\ simp [Once next_cases] \\ strip_tac \\ gvs [])
+    \\ drule_all eval_wh_Cons \\ rw [] \\ fs []
+    \\ fs [Once app_bisimilarity_iff])
+  THEN1
+   (qsuff_tac ‘∃m1 f1. eval_wh y = wh_Constructor "Bind" [m1;f1] ∧
+                       m ≃ m1 ∧ f ≃ f1’
+    THEN1 (rw [] \\ simp [Once next_cases]
+           \\ first_x_assum irule \\ fs []
+           \\ goal_assum (first_assum o mp_then Any mp_tac) \\ fs [])
+    \\ cheat)
+  THEN1
+   (qsuff_tac ‘eval_wh y = wh_Diverge’
+    THEN1 (simp [Once next_cases])
+    \\ cheat)
+  \\ cheat
+QED
+
+Theorem next_lemma_alt[local] =
+  next_lemma |> SIMP_RULE std_ss [PULL_FORALL,AND_IMP_INTRO];
+
+Theorem next_det:
+  ∀x1 r1 r2. next x1 r1 ∧ next x1 r2 ==> r1 = r2
+Proof
+  qsuff_tac ‘∀x1 r1. next x1 r1 ⇒ ∀r2. next x1 r2 ==> r1 = r2’
+  THEN1 (rw [] \\ res_tac \\ fs [])
+  \\ ho_match_mp_tac next_ind \\ rw []
+  \\ pop_assum mp_tac
+  \\ simp [Once next_cases] \\ strip_tac \\ gvs []
+QED
+
+Theorem symmetric_LIST_REL:
+  ∀xs ys R. symmetric R ∧ LIST_REL R xs ys ⇒ LIST_REL R ys xs
+Proof
+  Induct \\ fs [PULL_EXISTS] \\ rw [symmetric_def]
+QED
+
+Theorem bisimilarity_IMP_semantics_eq:
+  ∀x y. x ≃ y ⇒ semantics x [] = semantics y []
+Proof
+  cheat (*
+  qsuff_tac ‘∀x y xs ys. x ≃ y ∧ LIST_REL (≃) xs ys ⇒
+                         semantics x xs = semantics y ys’
+  THEN1 (rw [] \\ first_x_assum match_mp_tac)
+  \\ fs [io_el_eqv] \\ fs [PULL_FORALL] \\ rpt gen_tac
+  \\ EVERY (map qid_spec_tac [‘ys’,‘xs’,‘y’,‘x’])
+  \\ completeInduct_on ‘LENGTH path’ \\ rw [] \\ fs [PULL_FORALL]
+  \\ fs [semantics_def]
+  \\ once_rewrite_tac [interp_def]
+  \\ qsuff_tac ‘
+    next_action (eval_wh x,xs) = next_action (eval_wh y,ys) ∨
+    ∃a new1 new2.
+      next_action (eval_wh x,xs) = Act a new1 ∧
+      next_action (eval_wh y,ys) = Act a new2 ∧
+      LIST_REL (≃) new1 new2’
+  THEN1
+   (strip_tac \\ fs []
+    \\ Cases_on ‘path’ \\ fs [io_el_def]
+    \\ ‘wh_Constructor "Ret" [Lit h] = eval_wh (Ret (Lit h))’ by fs [eval_wh_Cons]
+    \\ fs [] \\ first_x_assum irule \\ fs []
+    \\ match_mp_tac reflexive_app_bisimilarity \\ fs [])
+  \\ qpat_x_assum ‘∀x. _’ kall_tac
+  \\ fs [next_action_def]
+  \\ Cases_on ‘∃res. next (eval_wh x,xs) res’ \\ fs []
+  THEN1
+   (drule_all next_lemma_alt \\ strip_tac
+    \\ ‘∀r. next (eval_wh x,xs) r ⇔ r = res’ by metis_tac [next_det]
+    \\ ‘∀r. next (eval_wh y,ys) r ⇔ r = res2’ by metis_tac [next_det]
+    \\ fs [] \\ metis_tac [])
+  \\ Cases_on ‘∃res. next (eval_wh y,ys) res’ \\ fs []
+  \\ drule next_lemma_alt
+  \\ disch_then (qspecl_then [‘x’,‘xs’] mp_tac)
+  \\ reverse impl_tac THEN1 (rw [] \\ fs [])
+  \\ assume_tac symmetric_app_bisimilarity
+  \\ drule_all symmetric_LIST_REL \\ fs []
+  \\ fs [symmetric_def] *)
+QED
+
+val _ = export_theory();
